---
title: "Computational Mathematics - Discussion 14"
author: "Mary Anna Kivenson"
date: "November 23, 2019"
output:
  rmarkdown::html_document:
    
    theme: cosmo 
    highlight: zenburn
---

```{r setup, include=FALSE}
library(ggfortify)
library(ggplot2)
library(dplyr)
knitr::opts_chunk$set(echo = TRUE)
```


## Calculus Discussion 14

### Question 4 {.tabset}
Key Idea 8.8.1 gives the nth term of the Taylor series of common functions. Verify the formula given in the Key Idea by finding the first few terms of the Taylor series of the given functions and identifying a pattern.

![](https://github.com/mkivenson/Computational-Mathematics/blob/master/Discussions/Discussion%2014/Key%20Idea.PNG?raw=true)


**Taylor Series**

The following is the formula for a Taylor series for function f(x).

$$f(x) = f(a) + f'(a)(x-a) + \frac{f''(a)}{2!}(x-a)^2 +...+ \frac{f^n(a)}{n!}(x-a)^n$$

#### Derivatives

**f(x) = sin(x), c=0**

* f(0) = sin(0) = 0
* f'(x) = cos(x) ->  cos(0) = 1
* f''(x) = -sin(x) -> -sin(0) = 0
* f'''(x) = -cos(x) -> -cos(0) = -1
* f''''(x) = sin(x) -> sin(0) = 0


#### First term
According to the key idea image above, the first time for this series should be x. 

$$first= f(a) = f(0) = sin(0) = 0$$

Since the first term is 0, we evaluate the next term instead.

$$first = f'(a)(x-a) = 1$$

#### Second term
According to the key idea image above, the first time for this series should be x^3/3!. 


$$second = \frac{f''(a)}{2!}(x-a)^2 = \frac{x^2}{2!}$$

Since the this term is 0, we evaluate the next term instead.

$$second = \frac{-1}{3!}x^3 = \frac{-x^3}{3!}$$

#### Third term
All even terms will be equal to 0, so we evaluate the the term for n=5. 

$$third = \frac{1}{5!}x^5 = \frac{x^5}{5!}$$

#### Fourth term
All even terms will be equal to 0, so we evaluate the the term for n=7. 

$$fourth = \frac{-1}{7!}x^7 = \frac{-x^7}{7!}$$


#### Pattern
The taylor series has the following patterns:

* All even terms are equal to zero 
* Non-zero terms alternate signs
* Exponents and factorials are odd

$$ sinx = \sum(-1)^n \frac{x^{2n+1}}{(2n+1)!}$$